update

lib/Lib.Bitmap.fst
@@ -1,156 +1,38 @@
 module Lib.Bitmap
 
 open Lib.IntTypes
+open Lib.Sliceable
 
-(*** Bitmap ***)
-
+private val aux (t:inttype{unsigned t}) (l:secrecy_level) : (xN:sig (bits t){xN.t == uint_t t l})
 #push-options "--fuel 1 --ifuel 1"
+let aux t l =
+{ t = int_t t l
+; v = (fun x i -> FStar.UInt.nth #(bits t) (v x) i)
+; mk = (fun f -> mk_int (UInt.from_vec #(bits t) (FStar.Seq.init (bits t) f)))
+; mk_def = (fun f i -> ())
+; ones_ = Lib.IntTypes.ones t l
+; zeros_ = Lib.IntTypes.zeros t l
+; and_ = logand
+; xor_ = logxor
+; or_ = logor
+; not_ = lognot
+; zeros_spec = (fun i -> UInt.zero_nth_lemma #(bits t) i)
+; ones_spec = (fun i -> UInt.ones_nth_lemma #(bits t) i)
+; and_spec = (fun x y i -> logand_spec x y)
+; xor_spec = (fun x y i -> logxor_spec x y)
+; or_spec = (fun x y i -> logor_spec x y)
+; not_spec = (fun x i -> lognot_spec x)
+}
+#pop-options
 
-private val nth (#t:intt) (#l:secl) (x:int_t t l) (i:nat{i<bits t}) : bool
-let nth #t #l x i = UInt.nth #(bits t) (v x) i
+val bitmap (t:inttype{unsigned t}) (l:secrecy_level) (n:nat) : Type0
+let rec bitmap t l n = if n <= bits t then int_t t l else int_t t l * bitmap t l (n-bits t)
 
-let rec bitmap t l n =
-  if n <= bits t then
-    int_t t l
+val uN (t:inttype{unsigned t}) (l:secrecy_level) (n:nat) : (xN:sig n{xN.t == bitmap t l n})
+let rec uN t l n =
+  if n = bits t then
+    aux t l
+  else if n < bits t then
+    xN_rest (aux t l) n
   else
-    int_t t l * bitmap t l (n-bits t)
-
-let rec bitmap_v #t #l #n x i =
-  if n <= bits t then (
-    nth (x <: int_t t l) i
-  ) else (
-    let (fst, rst) : int_t t l * bitmap t l (n-bits t) = x in
-    if i < bits t then (
-      nth fst i
-    ) else (
-      bitmap_v rst (i-bits t)
-    )
-  )
-
-private val offset (#a:Type) (#m:nat) (f:(i:nat{i<m}) -> a) (off:nat) (i:nat{i<m-off}) : a
-let offset f off i = f (i+off)
-
-let rec bitmap_mk t l n f =
-  if n <= bits t then (
-    let r = UInt.from_vec #(bits t) (FStar.Seq.init (bits t) (fun i -> if i<n then f i else false)) in
-    mk_int r <: int_t t l
-  ) else (
-    let r = UInt.from_vec #(bits t) (FStar.Seq.init (bits t) f) in
-    (mk_int r, bitmap_mk t l (n-bits t) (offset #_ #n f (bits t)))
-    <: int_t t l * bitmap t l (n-bits t)
-  )
-
-let rec bitmap_mk_def t l n f i =
-  if i < bits t then
-    ()
-  else
-    bitmap_mk_def t l (n-bits t) (offset #_ #n f (bits t)) (i-bits t)
-
-let rec bitmap_ones #t #l #n =
-  if n <= bits t then
-    ones t l
-  else
-    ((ones t l <: int_t t l), bitmap_ones #t #l #(n-bits t))
-
-let rec bitmap_zeros #t #l #n =
-  if n <= bits t then
-    zeros t l
-  else
-    ((zeros t l <: int_t t l), bitmap_zeros #t #l #(n-bits t))
-
-let rec bitmap_xor #t #l #n x y =
-  if n <= bits t then (
-    let u : int_t t l = x in
-    let v : int_t t l = y in
-    logxor u v
-  ) else (
-    let (u, r) : int_t t l * bitmap t l (n-bits t) = x in
-    let (v, s) : int_t t l * bitmap t l (n-bits t) = y in
-    (logxor u v, bitmap_xor r s)
-  )
-
-let rec bitmap_and #t #l #n x y =
-  if n <= bits t then (
-    let u : int_t t l = x in
-    let v : int_t t l = y in
-    logand u v
-  ) else (
-    let (u, r) : int_t t l * bitmap t l (n-bits t) = x in
-    let (v, s) : int_t t l * bitmap t l (n-bits t) = y in
-    (logand u v, bitmap_and r s)
-  )
-
-let rec bitmap_or #t #l #n x y =
-  if n <= bits t then (
-    let u : int_t t l = x in
-    let v : int_t t l = y in
-    logor u v
-  ) else (
-    let (u, r) : int_t t l * bitmap t l (n-bits t) = x in
-    let (v, s) : int_t t l * bitmap t l (n-bits t) = y in
-    (logor u v, bitmap_or r s)
-  )
-
-let rec bitmap_not #t #l #n x =
-  if n <= bits t then (
-    let u : int_t t l = x in
-    lognot u
-  ) else (
-    let (u, r) : int_t t l * bitmap t l (n-bits t) = x in
-    (lognot u, bitmap_not r)
-  )
-
-let rec bitmap_ones_spec #t #l #n i =
-  if i < bits t then
-    ()
-  else
-    bitmap_ones_spec #t #l #(n-bits t) (i-bits t)
-
-let rec bitmap_zeros_spec #t #l #n i =
-  if i < bits t then
-    UInt.zero_nth_lemma #(bits t) i
-  else
-    bitmap_zeros_spec #t #l #(n-bits t) (i-bits t)
-
-let rec bitmap_xor_spec #t #l #n x y i =
-  if n <= bits t then
-    logxor_spec (x <: int_t t l) (y <: int_t t l)
-  else
-    let (u1, v1) : int_t t l * bitmap t l (n-bits t) = x in
-    let (u2, v2) : int_t t l * bitmap t l (n-bits t) = y in
-    if i < bits t then
-      logxor_spec u1 u2
-    else
-      bitmap_xor_spec #t #l #(n-bits t) v1 v2 (i-bits t)
-
-let rec bitmap_and_spec #t #l #n x y i =
-  if n <= bits t then
-    logand_spec (x <: int_t t l) (y <: int_t t l)
-  else
-    let (u1, v1) : int_t t l * bitmap t l (n-bits t) = x in
-    let (u2, v2) : int_t t l * bitmap t l (n-bits t) = y in
-    if i < bits t then
-      logand_spec u1 u2
-    else
-      bitmap_and_spec #t #l #(n-bits t) v1 v2 (i-bits t)
-
-let rec bitmap_or_spec #t #l #n x y i =
-  if n <= bits t then
-    logor_spec (x <: int_t t l) (y <: int_t t l)
-  else
-    let (u1, v1) : int_t t l * bitmap t l (n-bits t) = x in
-    let (u2, v2) : int_t t l * bitmap t l (n-bits t) = y in
-    if i < bits t then
-      logor_spec u1 u2
-    else
-      bitmap_or_spec #t #l #(n-bits t) v1 v2 (i-bits t)
-
-let rec bitmap_not_spec #t #l #n x i =
-  if n <= bits t then
-    lognot_spec (x <: int_t t l)
-  else
-    let (u, v) : int_t t l * bitmap t l (n-bits t) = x in
-    if i < bits t then
-      lognot_spec u
-    else
-      bitmap_not_spec #t #l #(n-bits t) v (i-bits t)
+    xN_concat (bits t) (n-bits t) (aux t l) (uN t l (n-bits t))
