lib/Lib.Sliceable.fst
@@ -1,17 +1,21 @@
 module Lib.Sliceable
 
-open FStar.Tactics
 open FStar.UInt
-//open FStar.FunctionalExtensionality
+open FStar.Tactics
 
 #set-options "--fuel 0 --ifuel 0"
 
-(*** xN and xNxM ***)
+(*** Helper functions ***)
 
 let (^) (a b:bool) : bool = (a && (not b)) || ((not a) && b)
 
-noeq type sig (n:nat) : Type =
-{ t: Type
+private val offset (#a:Type) (#m:nat) (f:(i:nat{i<m}) -> a) (off:nat) (i:nat{i<m-off}) : a
+let offset f off i = f (i+off)
+
+(*** xN and xNxM ***)
+
+noeq type sig (n:nat) =
+{ t:Type0
 ; v: t -> (i:nat{i<n}) -> bool
 ; mk: (i:nat{i<n} -> bool) -> t
 ; mk_def: f:(i:nat{i<n} -> bool) -> i:nat{i<n} -> Lemma (v (mk f) i == f i)
@@ -29,85 +33,77 @@ noeq type sig (n:nat) : Type =
 ; not_spec: x:t -> i:nat{i<n} -> Lemma (v (not_ x) i == not(v x i))
 }
 
-let ( &&& ) (#n:nat) (#xN:sig n) (x y:xN.t) : xN.t = xN.and_ x y
-let ( ^^^ ) (#n:nat) (#xN:sig n) (x y:xN.t) : xN.t = xN.xor_ x y
-let ( ||| ) (#n:nat) (#xN:sig n) (x y:xN.t) : xN.t = xN.or_ x y
-let ( ~~~ ) (#n:nat) (#xN:sig n) (x:xN.t) : xN.t = xN.not_ x
-let ones (#n:nat) (xN:sig n) : xN.t = xN.ones_
-let zeros (#n:nat) (xN:sig n) : xN.t = xN.zeros_
+val xN_mk_def (#n:nat) (xN:sig n) (f:(i:nat{i<n} -> bool)) (i:nat{i<n}) :
+  Lemma (xN.v (xN.mk f) i == f i)
+  [SMTPat (xN.v (xN.mk f) i)]
 
-let op_String_Access (#n:nat) (#xN:sig n) (x:xN.t) (i:nat{i<n}) : bool = xN.v x i
+val xN_ones_spec (#n:nat) (xN:sig n) (i:nat{i<n}) :
+  Lemma (xN.v xN.ones_ i == true)
+  [SMTPat (xN.v xN.ones_ i)]
 
-let xN_mk_def (#n:nat) (#xN:sig n) (f:(i:nat{i<n} -> bool)) (i:nat{i<n}) :
-  Lemma ((xN.mk f).[i] == f i)
-  [SMTPat (xN.mk f).[i]]
-  = xN.mk_def f i
+val xN_zeros_spec (#n:nat) (xN:sig n) (i:nat{i<n}) :
+  Lemma (xN.v xN.zeros_ i == false)
+  [SMTPat (xN.v xN.zeros_ i)]
 
-let xN_ones_spec (#n:nat) (#xN:sig n) (i:nat{i<n}) :
-  Lemma ((ones xN).[i] == true)
-  [SMTPat (ones xN).[i]]
-  = xN.ones_spec i
+val xN_and_spec (#n:nat) (xN:sig n) (x y:xN.t) (i:nat{i<n}) :
+  Lemma (xN.v (xN.and_ x y) i == (xN.v x i && xN.v y i))
+  [SMTPat (xN.v (xN.and_ x y) i)]
 
-let xN_zeros_spec (#n:nat) (#xN:sig n) (i:nat{i<n}) :
-  Lemma ((zeros xN).[i] == false)
-  [SMTPat (zeros xN).[i]]
-  = xN.zeros_spec i
+val xN_xor_spec (#n:nat) (xN:sig n) (x y:xN.t) (i:nat{i<n}) :
+  Lemma (xN.v (xN.xor_ x y) i == (xN.v x i ^ xN.v y i))
+  [SMTPat (xN.v (xN.xor_ x y) i)]
 
-let xN_and_spec (#n:nat) (#xN:sig n) (x y:xN.t) (i:nat{i<n}) :
-  Lemma ((x &&& y).[i] == (x.[i] && y.[i]))
-  [SMTPat (x &&& y).[i]]
-  = xN.and_spec x y i
+val xN_or_spec (#n:nat) (xN:sig n) (x y:xN.t) (i:nat{i<n}) :
+  Lemma (xN.v (xN.or_ x y) i == (xN.v x i || xN.v y i))
+  [SMTPat (xN.v (xN.or_ x y) i)]
 
-let xN_xor_spec (#n:nat) (#xN:sig n) (x y:xN.t) (i:nat{i<n}) :
-  Lemma ((x ^^^ y).[i] == (x.[i] ^ y.[i]))
-  [SMTPat (x ^^^ y).[i]]
-  = xN.xor_spec x y i
+val xN_not_spec (#n:nat) (xN:sig n) (x:xN.t) (i:nat{i<n}) :
+  Lemma (xN.v (xN.not_ x) i == not (xN.v x i))
+  [SMTPat (xN.v (xN.not_ x) i)]
 
-let xN_or_spec (#n:nat) (#xN:sig n) (x y:xN.t) (i:nat{i<n}) :
-  Lemma ((x ||| y).[i] == (x.[i] || y.[i]))
-  [SMTPat (x ||| y).[i]]
-  = xN.or_spec x y i
+let xN_mk_def xN f i = xN.mk_def f i
+let xN_ones_spec xN i = xN.ones_spec i
+let xN_zeros_spec xN i = xN.zeros_spec i
+let xN_and_spec xN x y i = xN.and_spec x y i
+let xN_xor_spec xN x y i = xN.xor_spec x y i
+let xN_or_spec xN x y i = xN.or_spec x y i
+let xN_not_spec xN x i = xN.not_spec x i
 
-let xN_not_spec (#n:nat) (#xN:sig n) (x:xN.t) (i:nat{i<n}) :
-  Lemma ((~~~ x).[i] == not x.[i])
-  [SMTPat (~~~x).[i]]
-  = xN.not_spec x i
-
-//TODO: declaring type of xNxM before definition doesn't work
-let rec xNxM (#n:nat) (xN:sig n) (m:nat) : Type = if m = 0 then unit else xN.t * xNxM xN (m-1)
+val xNxM (#n:nat) (xN:sig n) (m:nat) : Type0
+#push-options "--fuel 1 --ifuel 1"
+let rec xNxM xN m = if m = 0 then unit else xN.t * xNxM xN (m-1)
+#pop-options
 
 val index (#n:nat) (#xN:sig n) (#m:nat) (x:xNxM xN m) (i:nat{i<m}) : xN.t
-#push-options "--fuel 1"
+#push-options "--ifuel 1 --fuel 1"
 let rec index #n #xN #m x i =
 if m = 0 then
   ()
 else
   let (u, v) : xN.t * xNxM xN (m-1) = x in
-  if i = 0 then
+  if i = m-1 then
     u
   else
-    index v (i-1)
+    index v i
 #pop-options
-
-private val offset (#a:Type) (#m:nat) (f:(i:nat{i<m}) -> a) (off:nat) (i:nat{i<m-off}) : a
-let offset f off i = f (i+off)
 
 val xNxM_mk (#n:nat) (xN:sig n) (m:nat) (f:(i:nat{i<m} -> xN.t)) : xNxM xN m
 #push-options "--fuel 1"
 let rec xNxM_mk xN m f =
-  if m = 0 then () else (f 0, xNxM_mk xN (m-1) (offset #_ #m f 1))
+  if m = 0 then () else (f (m-1), xNxM_mk xN (m-1) f)
 #pop-options
-
 
 val xNxM_mk_def (#n:nat) (xN:sig n) (m:nat) (f:(i:nat{i<m} -> xN.t)) (i:nat{i<m}) :
   Lemma (index (xNxM_mk xN m f) i == f i)
   [SMTPat (index (xNxM_mk xN m f) i)]
 #push-options "--fuel 1"
 let rec xNxM_mk_def xN m f i =
-  if i = 0 then
+  if m = 0 then
+    ()
+  else if i = m-1 then
     ()
   else
-    xNxM_mk_def xN (m-1) (offset #_ #m f 1) (i-1)
+    xNxM_mk_def xN (m-1) f i
 #pop-options
 
 val xNxM_eq_intro (#n:nat) (#xN:sig n) (#m:nat) (x y:xNxM xN m) :
@@ -121,10 +117,52 @@ let rec xNxM_eq_intro #n #xN #m x y =
   else
     let (a, u) : xN.t * xNxM xN (m-1) = x in
     let (b, v) : xN.t * xNxM xN (m-1) = y in
-    assert (forall (i:nat{i<m-1}). index u i == index x (i+1));
+    assert (forall (i:nat{i<m-1}). index u i == index x i);
     xNxM_eq_intro u v;
-    //assert (index x 0 == a);
-    assert (index y 0 == b)
+    //assert (index x (m-1) == a);
+    assert (index y (m-1) == b)
+#pop-options
+
+val xN_rest (#n:nat) (xN:sig n) (m:nat{m<=n}) : sig m
+let xN_rest (#n:nat) (xN:sig n) (m:nat{m<=n}) : sig m =
+{ t = xN.t
+; v = xN.v
+; mk = (fun f -> xN.mk (fun i -> if i < m then f i else false))
+; mk_def = (fun f i -> xN.mk_def (fun i -> if i < m then f i else false) i)
+; ones_ = xN.ones_
+; zeros_ = xN.zeros_
+; and_ = xN.and_
+; xor_ = xN.xor_
+; or_ = xN.or_
+; not_ = xN.not_
+; ones_spec = xN.ones_spec
+; zeros_spec = xN.zeros_spec
+; and_spec = xN.and_spec
+; xor_spec = xN.xor_spec
+; or_spec = xN.or_spec
+; not_spec = xN.not_spec
+}
+
+val xN_concat (#n:nat) (xN:sig n) (#m:nat) (xM:sig m) : sig (n+m)
+#push-options "--fuel 1 --ifuel 1"
+let xN_concat (#n:nat) (xN:sig n) (#m:nat) (xM:sig m) : sig (n+m) =
+{ t = xN.t * xM.t
+; v = (fun (x, y) i -> if i < n then xN.v x i else xM.v y (i-n))
+; mk = (fun f -> (xN.mk f), xM.mk (offset #_ #(n+m) f n))
+; mk_def = (fun f i -> if i < n then xN.mk_def f i else xM.mk_def (offset #_ #(n+m) f n) (i-n))
+; ones_ = (xN.ones_, xM.ones_)
+; zeros_ = (xN.zeros_, xM.zeros_)
+; and_ = (fun (x1, y1) (x2, y2) -> (xN.and_ x1 x2, xM.and_ y1 y2))
+; xor_ = (fun (x1, y1) (x2, y2) -> (xN.xor_ x1 x2, xM.xor_ y1 y2))
+; or_ = (fun (x1, y1) (x2, y2) -> (xN.or_ x1 x2, xM.or_ y1 y2))
+; not_ = (fun (x, y) -> (xN.not_ x, xM.not_ y))
+; ones_spec = (fun i -> if i < n then xN.ones_spec i else xM.ones_spec (i-n))
+; zeros_spec = (fun i -> if i < n then xN.zeros_spec i else xM.zeros_spec (i-n))
+; and_spec = (fun (x1, y1) (x2, y2) i -> if i < n then xN.and_spec x1 x2 i else xM.and_spec y1 y2 (i-n))
+; xor_spec = (fun (x1, y1) (x2, y2) i -> if i < n then xN.xor_spec x1 x2 i else xM.xor_spec y1 y2 (i-n))
+; or_spec = (fun (x1, y1) (x2, y2) i -> if i < n then xN.or_spec x1 x2 i else xM.or_spec y1 y2 (i-n))
+; not_spec = (fun (x, y) i -> if i < n then xN.not_spec x i else xM.not_spec y (i-n))
+}
 #pop-options
 
 (*** u1 and u1xM ***)
@@ -151,24 +189,50 @@ let u1 : sig 1 =
 val u1_of_bool (b:bool) : u1.t
 let u1_of_bool b = u1.mk (fun 0 -> b)
 
-val u1_of_bool_def (b:bool) : Lemma ((u1_of_bool b).[0] == b) [SMTPat (u1_of_bool b).[0]]
+val u1_of_bool_def (b:bool) : Lemma (u1.v (u1_of_bool b) 0 == b) [SMTPat (u1.v (u1_of_bool b) 0)]
 let u1_of_bool_def b = ()
 
-// TODO
-let u1xM (m:nat) : Type = xNxM u1 m
+let u1xM (m:nat) : Type0 = xNxM u1 m
+
+val u1xM_eq (#m:nat) (a b:u1xM m) : bool
+#push-options "--fuel 1 --ifuel 1"
+let rec u1xM_eq #m a b =
+  if m = 0 then
+    true
+  else
+    let (x1, y1) = a <: u1.t * u1xM (m-1) in
+    let (x2, y2) = b <: u1.t * u1xM (m-1) in
+    if x1 = x2 then u1xM_eq y1 y2 else false
+#pop-options
+
+val u1xM_eq_lemma (#m:nat) (a b:u1xM m) : Lemma (requires u1xM_eq a b) (ensures a == b)
+#push-options "--fuel 1 --ifuel 1"
+let rec u1xM_eq_lemma #m a b =
+  if m = 0 then
+    ()
+  else
+    let (x1, y1) = a <: u1.t * u1xM (m-1) in
+    let (x2, y2) = b <: u1.t * u1xM (m-1) in
+    u1xM_eq_lemma y1 y2
+#pop-options
 
 val u1xM_mk (m:nat) (f:(i:nat{i<m} -> bool)) : u1xM m
 let u1xM_mk m f = xNxM_mk _ _ (fun i -> u1_of_bool (f i))
 
 val column (#n:nat) (#xN:sig n) (#m:nat) (j:nat{j<n}) (x:xNxM xN m) : u1xM m
 let column j x =
-  let aux1 i k : bool = (index x i).[j] in
+  let aux1 i k : bool = (_).v (index x i) j in
   let aux2 i : u1.t = u1.mk (aux1 i) in
   xNxM_mk u1 _ aux2
 
+val column_def (#n:nat) (#xN:sig n) (#m:nat) (j:nat{j<n}) (x:xNxM xN m) (i:nat{i<m}) :
+  Lemma (index (column j x) i == (_).v (index x i) j)
+  [SMTPat (index (column j x) i)]
+let column_def j x i = ()
+
 val column_lemma (#n:nat) (#xN:sig n) (#m:nat) (x:xNxM xN m) (i:nat{i<m}) (j:nat{j<n}) :
-  Lemma ( (index (column j x) i).[0] == (index x i).[j] )
-  [SMTPat (index (column j x) i).[0]]
+  Lemma ( u1.v (index (column j x) i) 0 == xN.v (index x i) j )
+  [SMTPat (u1.v (index (column j x) i) 0)]
 let column_lemma x i j = ()
 
 val column_column (#m:nat) (x:u1xM m) :
@@ -178,10 +242,8 @@ let column_column x = xNxM_eq_intro (column 0 x) x
 
 (*** Sliceability ***)
 
-//TODO: broken
-//val sliceable (#m #m':nat) (f:(#n:nat -> #xN:sig n -> xNxM xN m -> xNxM xN m')) : Type0
-//let sliceable #m #m' f =
-let sliceable (#m #m':nat) (f:(#n:nat -> #xN:sig n -> xNxM xN m -> xNxM xN m')) : Type0 =
+val sliceable (#m #m':nat) (f:(#n:nat -> #xN:sig n -> xNxM xN m -> xNxM xN m')) : Type0
+let sliceable #m #m' f =
   forall (n:nat) (xN:sig n) (x:xNxM xN m) (j:nat{j<n}).
   ( column j (f x) == f (column j x))
 
@@ -197,22 +259,12 @@ let sliceable_intro f pr =
     )
   )
 
-val sliceable_elim
+val sliceable_def
   (#m #m':nat)
   (f:(#n:nat -> #xN:sig n -> xNxM xN m -> xNxM xN m'){sliceable f})
-  (#n:nat) (#xN:sig n) (x:xNxM xN m)
-  (j:nat{j<n})
-  : Lemma ( column j (f x) == f (column j x) )
-let sliceable_elim f x j = ()
-
-val sliceable_comp
-  (#m1 #m2 #m3:nat)
-  (f1:(#n:nat -> #xN:sig n -> xNxM xN m1 -> xNxM xN m2))
-  (f2:(#n:nat -> #xN:sig n -> xNxM xN m2 -> xNxM xN m3))
-  : Lemma
-    (requires sliceable f1 /\ sliceable f2)
-    (ensures sliceable (fun x -> f2 (f1 x)))
-let sliceable_comp f1 f2 = ()
+  : Lemma (forall (#n:nat) (#xN:sig n) (x:xNxM xN m) (j:nat{j<n}). column j (f x) == f (column j x))
+    [SMTPat (sliceable f)]
+let sliceable_def f = ()
 
 val sliceable_feq
   (#m #m':nat)
@@ -222,6 +274,32 @@ val sliceable_feq
     (requires forall (n:nat) (xN:sig n) (x:xNxM xN m). f x == g x)
     (ensures sliceable g)
 let sliceable_feq f g = ()
+
+val reduce_output
+  (#m #m':nat)
+  (f:(#n:nat -> #xN:sig n -> xNxM xN m -> xNxM xN m'))
+  (m'':nat) (r:(i:nat{i<m''} -> j:nat{j<m'}))
+  : #n:nat -> #xN:sig n -> xNxM xN m -> xNxM xN m''
+let reduce_output f m'' r x = xNxM_mk _ _ (fun i -> index (f x) (r i))
+
+val reduce_output_def
+  (#m #m':nat)
+  (f:(#n:nat -> #xN:sig n -> xNxM xN m -> xNxM xN m'))
+  (m'':nat) (r:(i:nat{i<m''} -> j:nat{j<m'}))
+  (#n:nat) (#xN:sig n) (x:xNxM xN m) (i:nat{i<m''})
+  : Lemma (index (reduce_output f m'' r x) i == index (f x) (r i))
+  [SMTPat (index (reduce_output f m'' r x) i)]
+let reduce_output_def f m'' r x i = ()
+
+val reduce_output_sliceable
+  (#m #m':nat)
+  (f:(#n:nat -> #xN:sig n -> xNxM xN m -> xNxM xN m'){sliceable f})
+  (m'':nat{m''<=m'}) (r:(i:nat{i<m''} -> j:nat{j<m'}))
+  : Lemma (sliceable (reduce_output f m'' r))
+  [SMTPat (sliceable (reduce_output f m'' r))]
+let reduce_output_sliceable f m'' r =
+  sliceable_intro (reduce_output f m'' r)
+    (fun x j -> xNxM_eq_intro (reduce_output f m'' r (column j x)) (column j (reduce_output f m'' r x)))
 
 (*** Circuits ***)
 
@@ -241,91 +319,60 @@ val circuit_def (#m #m':nat) (circ:circuit m m') (#n:nat) (#xN:sig n) (x:xNxM xN
 let rec circuit_def circ x i =
   match circ i with
   | Input j -> index x j
-  | Ones -> ones _
-  | Zeros -> zeros _
-  | Xor a b -> circuit_def circ x a ^^^ circuit_def circ x b
-  | And a b -> circuit_def circ x a &&& circuit_def circ x b
-  | Or a b -> circuit_def circ x a ||| circuit_def circ x b
-  | Not a -> ~~~(circuit_def circ x a)
+  | Ones -> (_).ones_
+  | Zeros -> (_).zeros_
+  | Xor a b -> (_).xor_ (circuit_def circ x a) (circuit_def circ x b)
+  | And a b -> (_).and_ (circuit_def circ x a) (circuit_def circ x b)
+  | Or a b -> (_).or_ (circuit_def circ x a) (circuit_def circ x b)
+  | Not a -> (_).not_ (circuit_def circ x a)
 #pop-options
 
-[@"opaqe_to_smt"]
-noeq
-type foo
-  (#m #m':nat) (circ:circuit m m')
-  (#n:nat) (#xN:sig n) (x:xNxM xN m)
-  (i:nat{i<m'}) =
-  | Foo : (u:xN.t{u == circuit_def circ x i}) -> foo circ x i
-
-[@"opaque_to_smt"]
-val circuit_input
-  (#m #m':nat) (#circ:circuit m m')
-  (#n:nat) (#xN:sig n) (#x:xNxM xN m)
-  (#c:nat{c<m'})
-  (j:nat{j<m})
-  : Pure (foo circ x c) (requires circ c == Input j) (ensures fun _ -> True)
-
-[@"opaque_to_smt"]
-val circuit_ones
-  (#m #m':nat) (#circ:circuit m m')
-  (#n:nat) (#xN:sig n) (#x:xNxM xN m)
-  (#c:nat{c<m'})
-  : Pure (foo circ x c) (requires circ c == Ones) (ensures fun _ -> True)
-
-[@"opaque_to_smt"]
-val circuit_zeros
-  (#m #m':nat) (#circ:circuit m m')
-  (#n:nat) (#xN:sig n) (#x:xNxM xN m)
-  (#c:nat{c<m'})
-  : Pure (foo circ x c) (requires circ c == Zeros) (ensures fun _ -> True)
-
-[@"opaque_to_smt"]
-val circuit_and
-  (#m #m':nat) (#circ:circuit m m')
-  (#n:nat) (#xN:sig n) (#x:xNxM xN m)
-  (#c:nat{c<m'})
-  (#a:nat{a<c}) (u:foo circ x a)
-  (#b:nat{b<c}) (v:foo circ x b)
-  : Pure (foo circ x c) (requires circ c == And a b) (ensures fun _ -> True)
-
-[@"opaque_to_smt"]
-val circuit_xor
-  (#m #m':nat) (#circ:circuit m m')
-  (#n:nat) (#xN:sig n) (#x:xNxM xN m)
-  (#c:nat{c<m'})
-  (#a:nat{a<c}) (u:foo circ x a)
-  (#b:nat{b<c}) (v:foo circ x b)
-  : Pure (foo circ x c) (requires circ c == Xor a b) (ensures fun _ -> True)
-
-[@"opaque_to_smt"]
-val circuit_or
-  (#m #m':nat) (#circ:circuit m m')
-  (#n:nat) (#xN:sig n) (#x:xNxM xN m)
-  (#c:nat{c<m'})
-  (#a:nat{a<c}) (u:foo circ x a)
-  (#b:nat{b<c}) (v:foo circ x b)
-  : Pure (foo circ x c) (requires circ c == Or a b) (ensures fun _ -> True)
-
-[@"opaque_to_smt"]
-val circuit_not
-  (#m #m':nat) (#circ:circuit m m')
-  (#n:nat) (#xN:sig n) (#x:xNxM xN m)
-  (#c:nat{c<m'})
-  (#a:nat{a<c}) (u:foo circ x a)
-  : Pure (foo circ x c) (requires circ c == Not a) (ensures fun _ -> True)
-
-#push-options "--fuel 1"
-let circuit_input #_ #_ #_ #_ #_ #x #_ j = Foo (index x j)
-let circuit_ones #_ #_ #_ #_ #_ #_ #_ = Foo (ones _)
-let circuit_zeros #_ #_ #_ #_ #_ #_ #_ = Foo (zeros _)
-let circuit_and u v = Foo (Foo?.u u &&& Foo?.u v)
-let circuit_xor u v = Foo (Foo?.u u ^^^ Foo?.u v)
-let circuit_or u v = Foo (Foo?.u u ||| Foo?.u v)
-let circuit_not u = Foo (~~~(Foo?.u u))
+val circuit_def_lemma (#m #m':nat) (circ:circuit m m') (#n:nat) (#xN:sig n) (x:xNxM xN m) (i:nat{i<m'-1}) :
+  Lemma (circuit_def #_ #(m'-1) circ x i == circuit_def #_ #m' circ x i)
+  [SMTPat (circuit_def #m #m' circ x i)]
+#push-options "--fuel 1 --ifuel 1"
+let rec circuit_def_lemma circ x i =
+  match circ i with
+  | Input j -> ()
+  | Ones -> ()
+  | Zeros -> ()
+  | Xor a b -> circuit_def_lemma circ x a; circuit_def_lemma circ x b
+  | And a b -> circuit_def_lemma circ x a; circuit_def_lemma circ x b
+  | Or a b -> circuit_def_lemma circ x a; circuit_def_lemma circ x b
+  | Not a -> circuit_def_lemma circ x a
 #pop-options
 
 val circuit_spec (#m #m':nat) (circ:circuit m m') (#n:nat) (#xN:sig n) (x:xNxM xN m) : xNxM xN m'
-let circuit_spec #_ #m' circ #_ #xN x = xNxM_mk xN m' (circuit_def circ x)
+let circuit_spec circ x = xNxM_mk _ _ (circuit_def circ x)
+
+val circuit_spec_lemma (#m #m':nat) (circ:circuit m m') (#n:nat) (#xN:sig n) (x:xNxM xN m) (i:nat{i<m'}) :
+  Lemma (index (circuit_spec circ x) i == circuit_def circ x i)
+  [SMTPat (index (circuit_spec circ x) i)]
+let circuit_spec_lemma circ x i = ()
+
+val circuit_spec' (#m #m':nat) (circ:circuit m m') (#n:nat) (#xN:sig n) (x:xNxM xN m) : (y:xNxM xN m'{y == circuit_spec circ x})
+#push-options "--fuel 1 --ifuel 1"
+let rec circuit_spec' #m #m' circ #n #xN x =
+  if m' = 0 then
+    ()
+  else (
+    let _ : (i:nat{i<m'}) = m'-1 in
+    let y : xNxM xN (m'-1) = circuit_spec' #_ #(m'-1) circ x in
+    let w : (w:xN.t{w == circuit_def circ x (m'-1)}) =
+      match circ (m'-1) with
+      | Input j -> index x j
+      | Ones -> (_).ones_
+      | Zeros -> (_).zeros_
+      | Xor a b -> (_).xor_ (index y a) (index y b)
+      | And a b -> (_).and_ (index y a) (index y b)
+      | Or a b -> (_).or_ (index y a) (index y b)
+      | Not a -> (_).not_ (index y a)
+    in
+    let z : xNxM xN m' = ((w <: xN.t), y) in
+    xNxM_eq_intro z (circuit_spec circ x);
+    z
+  )
+#pop-options
 
 private val sliceable_circuit_lemma
   (#m #m':nat)
@@ -335,7 +382,7 @@ private val sliceable_circuit_lemma
   (x:xNxM xN m)
   (i:nat{i<m'})
   (j:nat{j<n})
-  : Lemma ( (circuit_def circ x i).[j] == (circuit_def circ (column j x) i).[0] )
+  : Lemma ( xN.v (circuit_def circ x i) j == u1.v (circuit_def circ (column j x) i) 0 )
 #push-options "--fuel 1 --ifuel 1"
 let rec sliceable_circuit_lemma circ x i j = match circ i with
   | Ones -> ()
@@ -358,6 +405,9 @@ let sliceable_circuit circ =
 
 (*** of_uint and to_uint ***)
 
+val to_uint_spec (#m:nat) (x:u1xM m) : uint_t m
+let to_uint_spec #m x = FStar.UInt.from_vec (FStar.Seq.init m (index x))
+
 val of_uint_spec (#m:nat) (p:uint_t m) : u1xM m
 #push-options "--fuel 1"
 let of_uint_spec #m p =
@@ -366,9 +416,6 @@ let of_uint_spec #m p =
   else
     u1xM_mk _ (FStar.UInt.nth p)
 #pop-options
-
-val to_uint_spec (#m:nat) (x:u1xM m) : uint_t m
-let to_uint_spec #m x = FStar.UInt.from_vec (FStar.Seq.init m (index x))
 
 val to_uint (#m:nat) (x:u1xM m) : (p:uint_t m{p == to_uint_spec x})
 let to_uint #m x =
@@ -389,21 +436,14 @@ let to_uint #m x =
   aux m
 
 val of_uint (#m:nat) (p:uint_t m) : (x:u1xM m{x == of_uint_spec p})
-#push-options "--fuel 1"
 let of_uint #m p =
-  let rec aux (j:nat{j<=m}) (q:uint_t j) : (x:u1xM j{x == of_uint_spec #j q}) =
-    if j = 0 then
-      ()
-    else (
-      let u : u1.t = q%2 = 1 in
-      let v : u1xM (j-1) = aux (j-1) (q/2) in
-      let x : u1xM j = (u, v) in
-      assume (x == of_uint_spec #j q);
-      x
-    )
+  let aux (q:uint_t m) (i:nat{i<m}) : (r:bool{r == FStar.UInt.nth p i}) =
+    admit ();
+    q / (pow2 i) % 2 = 1
   in
-  aux m p
-#pop-options
+  let x = u1xM_mk _ (aux p) in
+  xNxM_eq_intro x (of_uint_spec p);
+  x
 
 val to_uint_of_uint (#m:nat) (p:uint_t m) :
   Lemma (to_uint (of_uint p) == p)
@@ -421,34 +461,56 @@ let of_uint_to_uint x = xNxM_eq_intro (of_uint (to_uint x)) x
 
 (*** Bruteforce lemmas and tactics ***)
 
-private val bruteforce_aux (n:nat) (phi:(i:nat{i<n} -> bool)) : bool
-let rec bruteforce_aux n phi =
-  if n = 0 then true else phi (n-1) && bruteforce_aux (n-1) phi
-
-private val bruteforce_aux_lemma (n:nat) (phi:(i:nat{i<n} -> bool)) :
-  Lemma
-    (requires bruteforce_aux n phi)
-    (ensures forall (i:nat{i<n}). phi i)
-#push-options "--fuel 1"
-let rec bruteforce_aux_lemma n phi =
-  if n = 0 then () else bruteforce_aux_lemma (n-1) phi
-#pop-options
-
-val bruteforce (#n:nat) (phi:(i:uint_t n -> bool)) : bool
-let bruteforce #n phi = bruteforce_aux (pow2 n) phi
-
-val bruteforce_lemma (#n:nat) (phi:(i:uint_t n -> bool)) :
-  Lemma
-    (requires bruteforce phi)
-    (ensures forall (i:uint_t n). phi i)
-let bruteforce_lemma #n phi = bruteforce_aux_lemma (pow2 n) phi
-
 val forall_uint_lemma (#m:nat) (phi:u1xM m -> Type0) :
   Lemma
     (requires forall (i:uint_t m). phi (of_uint i))
     (ensures forall x. phi x)
 let forall_uint_lemma phi =
   FStar.Classical.forall_intro (fun x -> of_uint_to_uint x <: Lemma (phi x))
+
+let bruteforce_aux (n:nat) (phi:(i:uint_t n -> bool)) :
+  Pure
+    bool
+    (requires True)
+    (fun r -> if r then forall (i:uint_t n). phi i else True)
+  =
+  let rec foo (n:nat) (phi:(i:nat{i<n} -> bool)) :
+    Pure
+      bool
+      (requires True)
+      (ensures fun r -> if r then forall (i:nat{i<n}). phi i else True)
+    = if n = 0 then true else phi (n-1) && foo (n-1) phi
+  in
+  foo (pow2 n) phi
+
+#push-options "--fuel 1 --ifuel 1"
+let bruteforce
+  (#m #m':nat)
+  (impl:(#n:nat -> #xN:sig n -> xNxM xN m -> xNxM xN m'))
+  (spec:(uint_t m -> uint_t m'))
+  : Pure
+    bool
+    (requires sliceable impl)
+    (ensures fun r ->
+      if r then
+        forall (n:nat) (xN:sig n) (x:xNxM xN m) (j:nat{j<n}).
+        column j (impl x) == of_uint (spec (to_uint (column j x)))
+      else
+        True
+    )
+  =
+  let phi0 (x:u1xM m) : Type0 = impl x == of_uint (spec (to_uint x)) in
+  let phi1 (i:uint_t m) : bool = u1xM_eq (impl (of_uint i)) (of_uint (spec i)) in
+  let r = bruteforce_aux m phi1 in
+  if r then (
+    FStar.Classical.forall_intro (fun (i:uint_t m) ->
+      u1xM_eq_lemma (impl (of_uint i)) (of_uint (spec i))
+      <: Lemma (impl (of_uint i) == of_uint (spec i))
+    );
+    forall_uint_lemma phi0;
+    true
+  ) else false
+#pop-options
 
 val nat_ind
   (n:pos)
